{-# OPTIONS --rewriting #-}

module A201802.WIP.LR3 where

open import A201801.Prelude
open import A201801.Category
open import A201801.Fin
open import A201801.FinLemmas
open import A201801.Vec
open import A201801.VecLemmas
open import A201801.AllVec

open import A201802.LR0
open import A201802.LR0Lemmas
open import A201802.LR1

open import A201802.LR2 -- TODO: which LR2?



postulate
  oops : ∀ {ℓ} → {X : Set ℓ} → X


--------------------------------------------------------------------------------


-- `SN _ A` is the strong normalisation predicate on terms at type `A`.
mutual
  SN : Term 0 → Type → Set
  SN M A = ∙ ⊢ M ⦂ A × M ⇓ × SN! M A

  SN! : Term 0 → Type → Set
  SN! M 𝔹       = ⊤
  SN! M (A ∨ B) = oops
  SN! M 𝟘       = ⊥
  SN! M 𝟙       = ⊤
  SN! M (A ∧ B) = SN (FST M) A × SN (SND M) B
  SN! M (A ⊃ B) = ∀ {N} → SN N A → SN (APP M N) B


-- Every SN term is well-typed.
derp : ∀ {A M} → SN M A
               → ∙ ⊢ M ⦂ A
derp (𝒟 , M⇓ , s!) = 𝒟


--------------------------------------------------------------------------------


-- `SNs _ Γ` is the strong normalisation predicate on substitutions at all types `Γ`.
SNs : ∀ {g} → (τ : Terms 0 g) → Types g → Set
SNs τ Γ = All (\ { (M , A) → SN M A }) (zip τ Γ)


-- Every SN substitution is well-typed.
derps : ∀ {g} → {τ : Terms 0 g} {Γ : Types g}
              → SNs τ Γ
              → ∙ ⊢ τ ⦂ Γ all
derps σ = maps derp σ


--------------------------------------------------------------------------------


-- -- Small-step reduction IN REVERSE preserves SN.
-- mutual
--   snpr↦ : ∀ {A M M′} → M ↦ M′ → ∙ ⊢ M ⦂ A → SN M′ A
--                       → SN M A
--   snpr↦ M↦M′ 𝒟 (𝒟′ , M′⇓ , s!′) = 𝒟 , hpr↦ M↦M′ M′⇓ , sn!pr↦ M↦M′ 𝒟 s!′

--   sn!pr↦ : ∀ {A M M′} → M ↦ M′ → ∙ ⊢ M ⦂ A → SN! M′ A
--                        → SN! M A
--   sn!pr↦ {𝔹}     M↦M′ 𝒟 ∙         = ∙
--   sn!pr↦ {A ∨ B} M↦M′ 𝒟 x         = oops
--   sn!pr↦ {𝟘}     M↦M′ 𝒟 ()
--   sn!pr↦ {𝟙}     M↦M′ 𝒟 ∙         = ∙
--   sn!pr↦ {A ∧ B} M↦M′ 𝒟 (s₁ , s₂) = snpr↦ (cong-fst M↦M′) (fst 𝒟) s₁ , snpr↦ (cong-snd M↦M′) (snd 𝒟) s₂
--   sn!pr↦ {A ⊃ B} M↦M′ 𝒟 f s       = snpr↦ (cong-app₁ M↦M′) (app 𝒟 (derp s)) (f s)


-- -- Iterated small-step reduction IN REVERSE preserves SN.
-- snpr⤅ : ∀ {A M M′} → M ⤅ M′ → ∙ ⊢ M ⦂ A → SN M′ A
--                     → SN M A
-- snpr⤅ done                𝒟 s = s
-- snpr⤅ (step M↦M″ M″⤅M′) 𝒟 s = snpr↦ M↦M″ 𝒟 (snpr⤅ M″⤅M′ (tp↦ M↦M″ 𝒟) s)


-- -- Big-step reduction IN REVERSE preserves SN.
-- snpr⇓ : ∀ {A M M′} → M ⇓ M′ → ∙ ⊢ M ⦂ A → SN M′ A
--                    → SN M A
-- snpr⇓ (M⤅M′ , VM′) 𝒟 s = snpr⤅ M⤅M′ 𝒟 s


-- --------------------------------------------------------------------------------


-- -- Small-step reduction preserves SN.
-- mutual
--   snp↦ : ∀ {A M M′} → M ↦ M′ → ∙ ⊢ M ⦂ A → SN M A
--                      → SN M′ A
--   snp↦ M↦M′ 𝒟 (_ , M⇓ , s!) = tp↦ M↦M′ 𝒟 , hp↦ M↦M′ M⇓ , sn!p↦ M↦M′ 𝒟 s!

--   sn!p↦ : ∀ {A M M′} → M ↦ M′ → ∙ ⊢ M ⦂ A → SN! M A
--                       → SN! M′ A
--   sn!p↦ {𝔹}     M↦M′ 𝒟 ∙         = ∙
--   sn!p↦ {A ∨ B} M↦M′ 𝒟 x         = oops
--   sn!p↦ {𝟘}     M↦M′ 𝒟 ()
--   sn!p↦ {𝟙}     M↦M′ 𝒟 ∙         = ∙
--   sn!p↦ {A ∧ B} M↦M′ 𝒟 (s₁ , s₂) = snp↦ (cong-fst M↦M′) (fst 𝒟) s₁ , snp↦ (cong-snd M↦M′) (snd 𝒟) s₂
--   sn!p↦ {A ⊃ B} M↦M′ 𝒟 f s       = snp↦ (cong-app₁ M↦M′) (app 𝒟 (derp s)) (f s)


-- -- Iterated small-step reduction preserves SN.
-- snp⤅ : ∀ {A M M′} → M ⤅ M′ → ∙ ⊢ M ⦂ A → SN M A
--                    → SN M′ A
-- snp⤅ done                𝒟 s = s
-- snp⤅ (step M↦M″ M″⤅M′) 𝒟 s = snp⤅ M″⤅M′ (tp↦ M↦M″ 𝒟) (snp↦ M↦M″ 𝒟 s)


-- -- Big-step reduction preserves SN.
-- snp⇓ : ∀ {A M M′} → M ⇓ M′ → ∙ ⊢ M ⦂ A → SN M A
--                   → SN M′ A
-- snp⇓ (M⤅M′ , VM′) 𝒟 s = snp⤅ M⤅M′ 𝒟 s


-- --------------------------------------------------------------------------------


-- -- If `M` is SN at type `A ⊃ B` and `N` is SN at type `A`, then `APP M N` is SN at type `B`.
-- sn-app : ∀ {A B M N} → SN M (A ⊃ B) → SN N A
--                      → SN (APP M N) B
-- sn-app (𝒟 , M⇓ , f) s = f s


-- -- If `M` is SN at type `A` and `N` is SN at type `B`, then `PAIR M N` is SN at type `A ∧ B`.
-- sn-pair : ∀ {A B M N} → SN M A → SN N B
--                       → SN (PAIR M N) (A ∧ B)
-- sn-pair s₁@(𝒟 , M⇓@(M′ , M⇓M′@(M⤅M′ , VM′)) , s!₁) s₂@(ℰ , N⇓@(N′ , N⇓N′@(N⤅N′ , VN′)) , s!₂)
--   = pair 𝒟 ℰ ,
--     halt-pair M⇓ N⇓ ,
--     snpr⇓ (big-red-fst-pair {{VM′}} {{VN′}} (congs-pair {{VM′}} {{VN′}} M⤅M′ N⤅N′)) (fst (pair 𝒟 ℰ)) (snp⤅ M⤅M′ 𝒟 s₁) ,
--     snpr⇓ (big-red-snd-pair {{VM′}} {{VN′}} ((congs-pair {{VM′}} {{VN′}} M⤅M′ N⤅N′))) (snd (pair 𝒟 ℰ)) (snp⤅ N⤅N′ ℰ s₂)


-- -- If `M` is SN at type `A ∧ B`, then `FST M` is SN at type `A`.
-- mutual
--   sn-fst : ∀ {A B M} → SN M (A ∧ B)
--                      → SN (FST M) A
--   sn-fst (𝒟 , M⇓ , s!) = fst 𝒟 , halt-fst 𝒟 M⇓ , sn!-fst s!

--   sn!-fst : ∀ {A B M} → SN! M (A ∧ B)
--                       → SN! (FST M) A
--   sn!-fst {𝔹}       _                      = ∙
--   sn!-fst {A₁ ∨ A₂} x                      = oops
--   sn!-fst {𝟘}       ()
--   sn!-fst {𝟙}       _                      = ∙
--   sn!-fst {A₁ ∧ A₂} ((ℰ , FST⇓ , s) , _)   = s
--   sn!-fst {A₁ ⊃ A₂} ((ℰ , FST⇓ , f) , _) s = f s


-- -- If `M` is SN at type `A ∧ B`, then `SND M` is SN at type `B`.
-- mutual
--   sn-snd : ∀ {A B M} → SN M (A ∧ B)
--                      → SN (SND M) B
--   sn-snd (𝒟 , M⇓ , s!) = snd 𝒟 , halt-snd 𝒟 M⇓ , sn!-snd s!

--   sn!-snd : ∀ {B A M} → SN! M (A ∧ B)
--                       → SN! (SND M) B
--   sn!-snd {𝔹}       _                      = ∙
--   sn!-snd {B₁ ∨ B₂} x                      = oops
--   sn!-snd {𝟘}       ()
--   sn!-snd {𝟙}       _                      = ∙
--   sn!-snd {B₁ ∧ B₂} (_ , (ℰ , SND⇓ , s))   = s
--   sn!-snd {B₁ ⊃ B₂} (_ , (ℰ , SND⇓ , f)) s = f s


-- -- If `M` is SN at type `𝟘`, then `ABORT M` is SN at type `C`.
-- mutual
--   sn-abort : ∀ {C M} → SN M 𝟘
--                      → SN (ABORT M) C
--   sn-abort {C} (𝒟 , M⇓ , s!) = abort 𝒟 , halt-abort 𝒟 M⇓ , sn!-abort {C} s!

--   sn!-abort : ∀ {C M} → SN! M 𝟘
--                       → SN! (ABORT M) C
--   sn!-abort {𝔹}     ()
--   sn!-abort {A ∨ B} x  = oops
--   sn!-abort {𝟘}     ()
--   sn!-abort {𝟙}     ()
--   sn!-abort {A ∧ B} ()
--   sn!-abort {A ⊃ B} () _


-- -- If `M` is SN at type `A`, then `LEFT M` is SN at type `A ∨ B`.
-- sn-left : ∀ {A B M} → SN M A
--                     → SN (LEFT M) (A ∨ B)
-- sn-left s@(𝒟 , M⇓@(M′ , M⇓M′@(M⤅M′ , VM′)) , s!) = left 𝒟 , halt-left M⇓ , oops


-- -- If `M` is SN at type `B`, then `RIGHT M` is SN at type `A ∨ B`.
-- sn-right : ∀ {A B M} → SN M B
--                      → SN (RIGHT M) (A ∨ B)
-- sn-right s@(𝒟 , M⇓@(M′ , M⇓M′@(M⤅M′ , VM′)) , s!) = right 𝒟 , halt-right M⇓ , oops


-- -- If `M` is SN at type `𝔹` and `N` is SN at type `C` and `O` is SN at type `C`, then `IF M N O` is SN at type `C`.
-- mutual
--   sn-if : ∀ {C M N O} → SN M 𝔹 → SN N C → SN O C
--                       → SN (IF M N O) C
--   sn-if (𝒟 , M⇓@(M′       , M⤅M′    , VM′)       , ∙) _              _              with tp⤅ M⤅M′ 𝒟
--   sn-if (𝒟 , M⇓@(LAM _    , _        , val-lam)   , ∙) _              _              | ()
--   sn-if (𝒟 , M⇓@(PAIR _ _ , _        , val-pair)  , ∙) _              _              | ()
--   sn-if (𝒟 , M⇓@(UNIT     , _        , val-unit)  , ∙) _              _              | ()
--   sn-if (𝒟 , M⇓@(LEFT _   , _        , val-left)  , ∙) _              _              | ()
--   sn-if (𝒟 , M⇓@(RIGHT _  , _        , val-right) , ∙) _              _              | ()
--   sn-if (𝒟 , M⇓@(TRUE     , M⤅TRUE  , val-true)  , ∙) (ℰ , N⇓ , s!₁) (ℱ , O⇓ , s!₂) | true  = if 𝒟 ℰ ℱ , halt-if 𝒟 M⇓ N⇓ O⇓ , sn!-if-true M⤅TRUE 𝒟 ℰ ℱ s!₁
--   sn-if (𝒟 , M⇓@(FALSE    , M⤅FALSE , val-false) , ∙) (ℰ , N⇓ , s!₁) (ℱ , O⇓ , s!₂) | false = if 𝒟 ℰ ℱ , halt-if 𝒟 M⇓ N⇓ O⇓ , sn!-if-false M⤅FALSE 𝒟 ℰ ℱ s!₂

--   sn!-if-true : ∀ {C M N O} → M ⤅ TRUE → ∙ ⊢ M ⦂ 𝔹 → ∙ ⊢ N ⦂ C → ∙ ⊢ O ⦂ C → SN! N C
--                             → SN! (IF M N O) C
--   sn!-if-true {𝔹}     M⤅TRUE 𝒟 ℰ ℱ ∙         = ∙
--   sn!-if-true {A ∨ B} M⤅TRUE 𝒟 ℰ ℱ x         = oops
--   sn!-if-true {𝟘}     M⤅TRUE 𝒟 ℰ ℱ ()
--   sn!-if-true {𝟙}     M⤅TRUE 𝒟 ℰ ℱ ∙         = ∙
--   sn!-if-true {A ∧ B} M⤅TRUE 𝒟 ℰ ℱ (s₁ , s₂) = snpr⤅ (congs-fst (reds-if-true M⤅TRUE done)) (fst (if 𝒟 ℰ ℱ)) s₁ ,
--                                                 snpr⤅ (congs-snd (reds-if-true M⤅TRUE done)) (snd (if 𝒟 ℰ ℱ)) s₂
--   sn!-if-true {A ⊃ B} M⤅TRUE 𝒟 ℰ ℱ f s       = snpr⤅ (congs-app₁ (reds-if-true M⤅TRUE done)) (app (if 𝒟 ℰ ℱ) (derp s)) (f s)

--   sn!-if-false : ∀ {C M N O} → M ⤅ FALSE → ∙ ⊢ M ⦂ 𝔹 → ∙ ⊢ N ⦂ C → ∙ ⊢ O ⦂ C → SN! O C
--                              → SN! (IF M N O) C
--   sn!-if-false {𝔹}     M⤅FALSE 𝒟 ℰ ℱ ∙         = ∙
--   sn!-if-false {A ∨ B} M⤅FALSE 𝒟 ℰ ℱ x         = oops
--   sn!-if-false {𝟘}     M⤅FALSE 𝒟 ℰ ℱ ()
--   sn!-if-false {𝟙}     M⤅FALSE 𝒟 ℰ ℱ ∙         = ∙
--   sn!-if-false {A ∧ B} M⤅FALSE 𝒟 ℰ ℱ (s₁ , s₂) = snpr⤅ (congs-fst (reds-if-false M⤅FALSE done)) (fst (if 𝒟 ℰ ℱ)) s₁ ,
--                                                   snpr⤅ (congs-snd (reds-if-false M⤅FALSE done)) (snd (if 𝒟 ℰ ℱ)) s₂
--   sn!-if-false {A ⊃ B} M⤅FALSE 𝒟 ℰ ℱ f s       = snpr⤅ (congs-app₁ (reds-if-false M⤅FALSE done)) (app (if 𝒟 ℰ ℱ) (derp s)) (f s)


-- -- XXX
-- mutual
--   sn-app-lam : ∀ {B g M N A} → {τ : Terms 0 g} → {{_ : Vals τ}} {{_ : Val N}}
--                              → ∙ ⊢ SUB τ (LAM M) ⦂ A ⊃ B → ∙ ⊢ N ⦂ A → SN (SUB (τ , N) M) B
--                              → SN (APP (LAM (SUB (LIFTS τ) M)) N) B
--   sn-app-lam {M = M} 𝒟 ℰ (𝒟′ , SUB⇓ , s!) =
--     let 𝒜 = app 𝒟 ℰ in
--       𝒜 , halt-app-lam {M = M} SUB⇓ , sn!-app-lam {M = M} 𝒜 s!

--   sn!-app-lam : ∀ {B g M N} → {τ : Terms 0 g} → {{_ : Vals τ}} {{_ : Val N}}
--                             → ∙ ⊢ APP (LAM (SUB (LIFTS τ) M)) N ⦂ B → SN! (SUB (τ , N) M) B
--                             → SN! (APP (LAM (SUB (LIFTS τ) M)) N) B
--   sn!-app-lam {𝔹}       {M = M} 𝒜 ∙         = ∙
--   sn!-app-lam {B₁ ∨ B₂} {M = M} 𝒜 x         = oops
--   sn!-app-lam {𝟘}       {M = M} 𝒜 ()
--   sn!-app-lam {𝟙}       {M = M} 𝒜 ∙         = ∙
--   sn!-app-lam {B₁ ∧ B₂} {M = M} 𝒜 (s₁ , s₂) = snpr↦ (cong-fst (red-app-lam {M = M})) (fst 𝒜) s₁ ,
--                                               snpr↦ (cong-snd (red-app-lam {M = M})) (snd 𝒜) s₂
--   sn!-app-lam {B₁ ⊃ B₂} {M = M} 𝒜 f s       = snpr↦ (cong-app₁ (red-app-lam {M = M})) (app 𝒜 (derp s)) (f s)


-- --------------------------------------------------------------------------------


-- mutual
--   gen-sn : ∀ {g M A} → {τ : Terms 0 g} {Γ : Types g} → {{_ : Vals τ}}
--                      → SNs τ Γ → Γ ⊢ M ⦂ A
--                      → SN (SUB τ M) A
--   gen-sn σ (var i)      = get σ (zip∋₂ i)
--   gen-sn σ (lam 𝒟)      = gen-sn-lam σ 𝒟
--   gen-sn σ (app 𝒟 ℰ)    = sn-app (gen-sn σ 𝒟) (gen-sn σ ℰ)
--   gen-sn σ (pair 𝒟 ℰ)   = sn-pair (gen-sn σ 𝒟) (gen-sn σ ℰ)
--   gen-sn σ (fst 𝒟)      = sn-fst (gen-sn σ 𝒟)
--   gen-sn σ (snd 𝒟)      = sn-snd (gen-sn σ 𝒟)
--   gen-sn σ unit         = unit , (UNIT , done , val-unit) , ∙
--   gen-sn σ (abort 𝒟)    = sn-abort (gen-sn σ 𝒟)
--   gen-sn σ (left 𝒟)     = sn-left (gen-sn σ 𝒟)
--   gen-sn σ (right 𝒟)    = sn-right (gen-sn σ 𝒟)
--   gen-sn σ (case 𝒟 ℰ ℱ) = gen-sn-case σ 𝒟 ℰ ℱ
--   gen-sn σ true         = true , (TRUE , done , val-true) , ∙
--   gen-sn σ false        = false , (FALSE , done , val-false) , ∙
--   gen-sn σ (if 𝒟 ℰ ℱ)   = sn-if (gen-sn σ 𝒟) (gen-sn σ ℰ) (gen-sn σ ℱ)

--   gen-sn-lam : ∀ {g M A B} → {τ : Terms 0 g} {Γ : Types g} → {{_ : Vals τ}}
--                            → SNs τ Γ → Γ , A ⊢ M ⦂ B
--                            → SN (LAM (SUB (LIFTS τ) M)) (A ⊃ B)
--   gen-sn-lam {M = M} {{Vτ}} σ 𝒟 =
--     let 𝒟′ = sub (derps σ) (lam 𝒟) in
--       𝒟′ , (LAM _ , done , val-lam) , (\ { s@(ℰ , (N′ , N⇓N′@(N⤅N′ , VN′)) , s!) →
--         let s′@(ℰ′ , _ , _) = snp⇓ N⇓N′ ℰ s in
--           snpr⤅ (congs-app₂ N⤅N′)
--                  (app 𝒟′ ℰ)
--                  (sn-app-lam {M = M} {{Vτ}} {{VN′}}
--                    𝒟′ ℰ′
--                    (gen-sn {{Vτ , VN′}} (σ , s′) 𝒟)) })


--   gen-sn-case : ∀ {g M N O A B C} → {τ : Terms 0 g} {Γ : Types g} → {{_ : Vals τ}}
--                                   → SNs τ Γ → Γ ⊢ M ⦂ A ∨ B → Γ , A ⊢ N ⦂ C → Γ , B ⊢ O ⦂ C
--                                   → SN (CASE (SUB τ M) (SUB (LIFTS τ) N) (SUB (LIFTS τ) O)) C
--   gen-sn-case {N = N} {O} {{Vτ}} σ 𝒟 ℰ ℱ with gen-sn σ 𝒟
--   gen-sn-case {N = N} {O} {{Vτ}} σ 𝒟 ℰ ℱ | s₁@(𝒟′ , (M′       , SUB⤅M′    , VM′)       , s₁!) with tp⤅ SUB⤅M′ 𝒟′
--   gen-sn-case {N = N} {O} {{Vτ}} σ 𝒟 ℰ ℱ | s₁@(𝒟′ , (LAM _    , _          , val-lam)   , s₁!) | ()
--   gen-sn-case {N = N} {O} {{Vτ}} σ 𝒟 ℰ ℱ | s₁@(𝒟′ , (PAIR _ _ , _          , val-pair)  , s₁!) | ()
--   gen-sn-case {N = N} {O} {{Vτ}} σ 𝒟 ℰ ℱ | s₁@(𝒟′ , (UNIT     , _          , val-unit)  , s₁!) | ()
--   gen-sn-case {N = N} {O} {{Vτ}} σ 𝒟 ℰ ℱ | s₁@(𝒟′ , (LEFT M″  , SUB⤅LEFT  , val-left {{VM″}})  , s₁!) | left _
--     = let step2 = gen-sn {M = N} {{Vτ , VM″}} (σ , {!s₁!}) ℰ in {!!}




-- --    = -- let x = snp⤅ SUB⤅LEFT {!!} {!!} in
-- --      let (ℰ′ , N⇓@(N′ , N⤅N′ , VN′) , s₂) = gen-sn (σ , {!s₁!}) ℰ in
-- --
-- --      snpr⤅ (congs-case SUB⤅LEFT)
-- --             (case 𝒟′ (sub (lifts (derps σ)) ℰ) (sub (lifts (derps σ)) ℱ))
-- --             (case (left 𝒟″) (sub (lifts (derps σ)) ℰ) (sub (lifts (derps σ)) ℱ) ,
-- --               halt-case-left {N = N} {O} N⇓ , {!!})
-- --
-- --    -- = let (ℰ′ , N⇓@(N′ , N⤅N′ , VN′) , s₂) = gen-sn (σ , unsn-left (snp⤅ SUB⤅LEFT 𝒟′ s₁)) ℰ in
-- --    --     sub (derps σ) (case 𝒟 ℰ ℱ) , (N′ , {!!} , {!!}) , {!!}
--   gen-sn-case {N = N} {O} σ 𝒟 ℰ ℱ | s₁@(𝒟′ , (RIGHT _  , SUB⤅RIGHT , val-right) , s!) | right 𝒟″
--     = {!!}



-- --    = sub (derps σ) (case 𝒟 ℰ ℱ) , ({!!} , {!!} , {!!}) , {!!}
--   gen-sn-case {N = N} {O} σ 𝒟 ℰ ℱ | s₁@(𝒟′ , (TRUE     , _          , val-true)  , s!) | ()
--   gen-sn-case {N = N} {O} σ 𝒟 ℰ ℱ | s₁@(𝒟′ , (FALSE    , _          , val-false) , s!) | ()

-- --    let (𝒟′ , ⇓M@(M′ , M⤅M′ , VM′) , s!) = gen-sn σ 𝒟 in
-- --      sub (derps σ) (case 𝒟 ℰ ℱ) , {!!} , {!!}


-- --------------------------------------------------------------------------------


-- -- Every well-typed term is SN.
-- sn : ∀ {A M} → ∙ ⊢ M ⦂ A
--              → SN M A
-- sn {A} {M} 𝒟 = subst (\ M′ → SN M′ A) (id-SUB M) (gen-sn ∙ 𝒟)


-- -- Every SN term terminates.
-- herp : ∀ {A M} → SN M A
--                → M ⇓
-- herp (𝒟 , M⇓ , s!) = M⇓


-- -- Every well-typed term terminates.
-- halt : ∀ {A M} → ∙ ⊢ M ⦂ A
--                → M ⇓
-- halt {A} 𝒟 = herp {A} (sn 𝒟)


-- --------------------------------------------------------------------------------
