module AltArtemovS4 where

open import Relation.Binary.PropositionalEquality using (_â‰¡_ ; refl)

import AltArtemov as ğœ†âˆ
import S4


forget : ğœ†âˆ.Ty â†’ S4.Ty
forget ğœ†âˆ.âŠ¥      = S4.âŠ¥
forget (A ğœ†âˆ.âŠƒ B) = forget A S4.âŠƒ forget B
forget (A ğœ†âˆ.âˆ§ B) = forget A S4.âˆ§ forget B
forget (x ğœ†âˆ.âˆ¶ A) = S4.â–¡ forget A


ğœ†âˆ-drop : âˆ€{A} â†’ ğœ†âˆ.âŠ© A â†’ ğœ†âˆ.Ty
ğœ†âˆ-drop {A} _ = A

S4-drop : âˆ€{A} â†’ S4.âŠ© A â†’ S4.Ty
S4-drop {A} _ = A


tI : âˆ€{A} â†’ forget (ğœ†âˆ-drop (ğœ†âˆ.tI {A})) â‰¡ S4-drop (S4.tI {forget A})
tI = refl

tIÂ² : âˆ€{A} â†’ forget (ğœ†âˆ-drop (ğœ†âˆ.tIÂ² {A})) â‰¡ S4-drop (S4.tIÂ² {forget A})
tIÂ² = refl


tK : âˆ€{A B} â†’ forget (ğœ†âˆ-drop (ğœ†âˆ.tK {A} {B})) â‰¡ S4-drop (S4.tK {forget A} {forget B})
tK = refl

tKÂ² : âˆ€{A B} â†’ forget (ğœ†âˆ-drop (ğœ†âˆ.tKÂ² {A} {B})) â‰¡ S4-drop (S4.tKÂ² {forget A} {forget B})
tKÂ² = refl


tS : âˆ€{A B C} â†’ forget (ğœ†âˆ-drop (ğœ†âˆ.tS {A} {B} {C})) â‰¡ S4-drop (S4.tS {forget A} {forget B} {forget C})
tS = refl

tSÂ² : âˆ€{A B C} â†’ forget (ğœ†âˆ-drop (ğœ†âˆ.tSÂ² {A} {B} {C})) â‰¡ S4-drop (S4.tSÂ² {forget A} {forget B} {forget C})
tSÂ² = refl


tE13 : âˆ€{A B} â†’ forget (ğœ†âˆ-drop (ğœ†âˆ.tE13 {A} {B})) â‰¡ S4-drop (S4.tE13 {forget A} {forget B})
tE13 = refl

tE14 : âˆ€{x y A B} â†’ forget (ğœ†âˆ-drop (ğœ†âˆ.tE14 {x} {y} {A} {B})) â‰¡ S4-drop (S4.tE14 {forget A} {forget B})
tE14 = refl
