module SimpleSTLC where

open import Data.Nat using (â„• ; zero ; suc ; _âŠ”_)
open import Data.Product using (_Ã—_) renaming (_,_ to âŸ¨_,_âŸ©)
open import Data.Vec using (Vec ; [] ; _âˆ·_ ; replicate)
open import Relation.Binary.PropositionalEquality using (_â‰¡_ ; refl)

infixl 9 ğ‘£_ ğ’—_
infixl 7 _âˆ˜_ _âˆ™_
infixr 5 ğœ†_ ğ€_
infixr 4 Â¬_
infixl 3 _,_ _â€_
infixr 2 _âŠƒ_
infixr 0 _âŠ¢_âˆ·_ âŠ©_âˆ·_


data Tm : â„• â†’ Set where
  ğ‘£_  : (x : â„•) â†’ Tm (suc x)
  ğœ†_  : âˆ€{x} â†’ Tm (suc x) â†’ Tm x
  _âˆ˜_ : âˆ€{x y} â†’ Tm x â†’ Tm y â†’ Tm (x âŠ” y)


module Demo where
  K : Tm 0
  K = ğœ† ğœ† ğ‘£ 1

  Kâ€² : Tm 1
  Kâ€² = ğœ† ğ‘£ 1

  S : Tm 0
  S = ğœ† ğœ† ğœ† (ğ‘£ 2 âˆ˜ ğ‘£ 0) âˆ˜ (ğ‘£ 1 âˆ˜ ğ‘£ 0)


data Ty : Set where
  _âŠƒ_ : Ty â†’ Ty â†’ Ty
  âŠ¥ : Ty


âŠ¤ : Ty
âŠ¤ = âŠ¥ âŠƒ âŠ¥

Â¬_ : Ty â†’ Ty
Â¬ A = A âŠƒ âŠ¥


data Cx : Set where
  âˆ…   : Cx
  _,_ : Cx â†’ Ty â†’ Cx


_â€_ : Cx â†’ Cx â†’ Cx
Î“ â€ âˆ…       = Î“
Î“ â€ (Î” , A) = Î“ â€ Î” , A


data _âˆˆ[_]_ : Ty â†’ â„• â†’ Cx â†’ Set where
  ğ™ : âˆ€{A Î“}
      â†’ A âˆˆ[ zero ] (Î“ , A)

  ğ’_ : âˆ€{A B x Î“}
      â†’ A âˆˆ[ x ] Î“
      â†’ A âˆˆ[ suc x ] (Î“ , B)


data _âŠ¢_âˆ·_ (Î“ : Cx) : âˆ€{x} â†’ Tm x â†’ Ty â†’ Set where
  ğ’—_ : âˆ€{i A}
      â†’ A âˆˆ[ i ] Î“
      â†’ Î“ âŠ¢ ğ‘£ i âˆ· A

  ğ€_ : âˆ€{x} {t : Tm (suc x)} {A B}
      â†’ Î“ , A âŠ¢ t âˆ· B
      â†’ Î“ âŠ¢ ğœ† t âˆ· (A âŠƒ B)

  _âˆ™_ : âˆ€{x y} {t : Tm x} {s : Tm y} {A B}
      â†’ Î“ âŠ¢ t âˆ· (A âŠƒ B)    â†’ Î“ âŠ¢ s âˆ· A
      â†’ Î“ âŠ¢ t âˆ˜ s âˆ· B


âŠ©_âˆ·_  : âˆ€{x} â†’ Tm x â†’ Ty â†’ Set
âŠ© t âˆ· A = âˆ€{Î“} â†’ Î“ âŠ¢ t âˆ· A


ğŸ : âˆ€{A Î“}
    â†’ A âˆˆ[ 0 ] (Î“ , A)
ğŸ = ğ™

ğŸ : âˆ€{A B Î“}
    â†’ A âˆˆ[ 1 ] (Î“ , A , B)
ğŸ = ğ’ ğŸ

ğŸ : âˆ€{A B C Î“}
    â†’ A âˆˆ[ 2 ] (Î“ , A , B , C)
ğŸ = ğ’ ğŸ


I : âˆ€{A}
    â†’ âŠ© ğœ† ğ‘£ 0 âˆ· A âŠƒ A
I = ğ€ ğ’— ğŸ

K : âˆ€{A B}
    â†’ âŠ© ğœ† ğœ† ğ‘£ 1 âˆ· A âŠƒ B âŠƒ A
K = ğ€ ğ€ ğ’— ğŸ

Kâ€² : âˆ€{A B Î“}
    â†’ Î“ , A âŠ¢ ğœ† ğ‘£ 1 âˆ· B âŠƒ A
Kâ€² = ğ€ ğ’— ğŸ

S : âˆ€{A B C}
    â†’ âŠ© ğœ† ğœ† ğœ† (ğ‘£ 2 âˆ˜ ğ‘£ 0) âˆ˜ (ğ‘£ 1 âˆ˜ ğ‘£ 0) âˆ· (A âŠƒ B âŠƒ C) âŠƒ (A âŠƒ B) âŠƒ A âŠƒ C
S = ğ€ ğ€ ğ€ (ğ’— ğŸ âˆ™ ğ’— ğŸ) âˆ™ (ğ’— ğŸ âˆ™ ğ’— ğŸ)
