{-# OPTIONS --sized-types #-}

module A201607.WIP2.BasicICML.Sketch2 where

open import A201607.BasicICML.Syntax.DyadicGentzen hiding (â„• ; ğŸ˜ ; ğŸ™) public

infixl 3 _+_
postulate
  â„• : Ty
  ğŸ˜ ğŸ™ ğŸš ğŸ› ğŸ : âˆ€ {Î“ Î”} â†’ Î“ â Î” âŠ¢ â„•
  _+_ : âˆ€ {Î“ Î”} â†’ Î“ â Î” âŠ¢ â„• â†’ Î“ â Î” âŠ¢ â„• â†’ Î“ â Î” âŠ¢ â„•

-- Letâ€™s say we have a simple expression referencing a free variable.

eâ‚ : âˆ€ {Î“ Î”} â†’ Î“ , â„• â Î” âŠ¢ â„•
eâ‚ = ğŸ™ + ğŸš + vâ‚€

-- We can partially normalise the expression without having to substitute the
-- variable away.

neâ‚ : âˆ€ {Î“ Î”} â†’ Î“ , â„• â Î” âŠ¢ â„•
neâ‚ = ğŸ› + vâ‚€

-- In ICML, we can quote expressions with free variables.  Therefore, if we can
-- check quoted expressions for Î±-equivalence, we can distinguish between the
-- original and the partially-normalised version of the expression.

qeâ‚ : âˆ€ {Î“ Î”} â†’ Î“ â Î” âŠ¢ [ âˆ… , â„• ] â„•
qeâ‚ = box (ğŸ™ + ğŸš + vâ‚€)

qneâ‚ : âˆ€ {Î“ Î”} â†’ Î“ â Î” âŠ¢ [ âˆ… , â„• ] â„•
qneâ‚ = box (ğŸ› + vâ‚€)

-- We can also consider the free variable as a reference to a previously
-- introduced definition, by replacing it with a free meta-variable.

eâ‚‚ : âˆ€ {Î“ Î”} â†’ Î“ â Î” , [ âˆ… ] â„• âŠ¢ â„•
eâ‚‚ = ğŸ™ + ğŸš + mvâ‚€ âˆ™

neâ‚‚ : âˆ€ {Î“ Î”} â†’ Î“ â Î” , [ âˆ… ] â„• âŠ¢ â„•
neâ‚‚ = ğŸ› + mvâ‚€ âˆ™

-- TODO: Unclear whether free meta-variables should or should not be listed in
-- the type of quoted expressions.

qeâ‚‚ : âˆ€ {Î“ Î”} â†’ Î“ â Î” , [ âˆ… ] â„• âŠ¢ [ âˆ… ] â„•
qeâ‚‚ = box (ğŸ™ + ğŸš + mvâ‚€ âˆ™)

qneâ‚‚ : âˆ€ {Î“ Î”} â†’ Î“ â Î” , [ âˆ… ] â„• âŠ¢ [ âˆ… ] â„•
qneâ‚‚ = box (ğŸ› + mvâ‚€ âˆ™)

-- Letâ€™s say we have previously introduced a definition of 3, and we want to
-- reference it in our expression in a manner similar to let-binding, that is:
--   let three = 3 in 1 + 2 + three

eâ‚ƒ : âˆ€ {Î“ Î”} â†’ Î“ â Î” âŠ¢ â„•
eâ‚ƒ = unbox {Î¨ = âˆ…} (box ğŸ›) (ğŸ™ + ğŸš + mvâ‚€ âˆ™)

neâ‚ƒ : âˆ€ {Î“ Î”} â†’ Î“ â Î” âŠ¢ â„•
neâ‚ƒ = unbox {Î¨ = âˆ…} (box ğŸ›) (ğŸ› + mvâ‚€ âˆ™)

qeâ‚ƒ : âˆ€ {Î“ Î”} â†’ Î“ â Î” âŠ¢ [ âˆ… ] â„•
qeâ‚ƒ = unbox {Î¨ = âˆ…} (box ğŸ›) (box (ğŸ™ + ğŸš + mvâ‚€ âˆ™))

qneâ‚ƒ : âˆ€ {Î“ Î”} â†’ Î“ â Î” âŠ¢ [ âˆ… ] â„•
qneâ‚ƒ = unbox {Î¨ = âˆ…} (box ğŸ›) (box (ğŸ› + mvâ‚€ âˆ™))

-- Now, we can achieve the expected result of splicing by performing one step
-- of reduction, or meta-variable substitution.

qeâ‚„ : âˆ€ {Î“ Î”} â†’ Î“ â Î” âŠ¢ [ âˆ… ] â„•
qeâ‚„ = box (ğŸ™ + ğŸš + ğŸ›)

qneâ‚„ : âˆ€ {Î“ Î”} â†’ Î“ â Î” âŠ¢ [ âˆ… ] â„•
qneâ‚„ = box (ğŸ› + ğŸ›)

-- Both of the above quoted expressions are nevertheless different from what we
-- would get by normalising before quoting (box-val).

qeâ‚… : âˆ€ {Î“ Î”} â†’ Î“ â Î” âŠ¢ [ âˆ… ] â„•
qeâ‚… = box ğŸ
