---
author:  P.Â Selinger
hauthor: Peter Selinger
year:    1992
title:   Friedmanâ€™s A-translation
lang:    en
card:
  - P.Â Selinger (1992)
  - '[Friedmanâ€™s A-translation
    ](https://www.mscs.dal.ca/~selinger/papers/friedman.pdf)'
  - Manuscript.
todo:
  - DOI missing
---

<style>
  pre {
    position: relative;
    left: 0;
    max-width: 100%;
    margin: 3.3rem 0 3.5rem 0;
  }
</style>


```
-- Mechanised by MiÃ«tek Bak
-- thanks to AndrÃ¡s, Ambrus, ames, drvink, Jesper, ncf, and roconnor
-- first-order predicate logic with one sort (naturals) and one predicate (equality)
-- variant with first-order structures for renaming and substitution

{-# OPTIONS --rewriting #-}

module mi.Selinger1992 where

open import mi.FOL public


----------------------------------------------------------------------------------------------------

-- TODO: statement of theorem 1


----------------------------------------------------------------------------------------------------

-- lemma 2

lem2 : âˆ€ {Ã k} {Î“ : FmÂ§ k} {A} â†’ Ã / Î“ âŠ¢ A â†’ PA / Î“ âŠ¢ A
lem2 (â€µvar i)                = â€µvar i
lem2 (â€µlam d)                = â€µlam (lem2 d)
lem2 (d â€µ$ e)                = lem2 d â€µ$ lem2 e
lem2 (â€µpair d e)             = â€µpair (lem2 d) (lem2 e)
lem2 (â€µfst d)                = â€µfst (lem2 d)
lem2 (â€µsnd d)                = â€µsnd (lem2 d)
lem2 (â€µleft d)               = â€µleft (lem2 d)
lem2 (â€µright d)              = â€µright (lem2 d)
lem2 (â€µeither c d e)         = â€µeither (lem2 c) (lem2 d) (lem2 e)
lem2 (â€µall refl d)           = â€µall refl (lem2 d)
lem2 (â€µunall t refl d)       = â€µunall t refl (lem2 d)
lem2 (â€µex t refl d)          = â€µex t refl (lem2 d)
lem2 (â€µletex refl refl d e)  = â€µletex refl refl (lem2 d) (lem2 e)
lem2 (â€µabortHA d)            = â€µabort (lem2 d)
lem2 (â€µmagicPA d)            = â€µmagicPA (lem2 d)
lem2 â€µrefl                   = â€µrefl
lem2 (â€µsym d)                = â€µsym (lem2 d)
lem2 (â€µtrans d e)            = â€µtrans (lem2 d) (lem2 e)
lem2 (â€µcong f i refl refl d) = â€µcong f i refl refl (lem2 d)
lem2 â€µdis                    = â€µdis
lem2 (â€µinj d)                = â€µinj (lem2 d)
lem2 (â€µind refl refl d e)    = â€µind refl refl (lem2 d) (lem2 e)
lem2 (â€µproj i refl)          = â€µproj i refl
lem2 (â€µcomp g Ï† refl)        = â€µcomp g Ï† refl
lem2 (â€µrec f g)              = â€µrec f g


----------------------------------------------------------------------------------------------------

-- quantifier-free formulas

data IsQFree {k} : Fm k â†’ Set where
  _â€µâŠƒ_ : âˆ€ {A B} (p : IsQFree A) (q : IsQFree B) â†’ IsQFree (A â€µâŠƒ B)
  _â€µâˆ§_ : âˆ€ {A B} (p : IsQFree A) (q : IsQFree B) â†’ IsQFree (A â€µâˆ§ B)
  _â€µâˆ¨_ : âˆ€ {A B} (p : IsQFree A) (q : IsQFree B) â†’ IsQFree (A â€µâˆ¨ B)
  â€µâŠ¥  : IsQFree â€µâŠ¥
  _â€µ=_ : âˆ€ {t u} â†’ IsQFree (t â€µ= u)

-- TODO: lemma 3
-- module _ where
--   open =-Reasoning
--
--   lem3 : âˆ€ {Ã k} {Î“ : FmÂ§ k} (A : Fm k) {{_ : IsQFree A}} â†’ Î£ (Prim k) Î» f â†’
--            Ã / Î“ âŠ¢ A â€µâ«— â€µfun f (tab â€µvar) â€µ= ğŸ˜
--   lem3 (A â€µâŠƒ B) = {!!}
--   lem3 (A â€µâˆ§ B) = {!!}
--   lem3 (A â€µâˆ¨ B) = {!!}
--   lem3 â€µâŠ¥      = sig
--                     (Æ’const 1)
--                     (â€µpair
--                       (â€µlam (abort 0))
--                       (â€µlam (â€µdis â€µ$ (â€µlam goal) â€µ$ 0)))
--                   where
--                     goal : âˆ€ {Ã k} {Î“ : FmÂ§ k} â†’
--                              Ã / Î“ , â€µfun (Æ’const 1) (tab â€µvar) â€µ= ğŸ˜ âŠ¢ ğ•Š ğŸ˜ â€µ= ğŸ˜
--                     goal = begin
--                              ğ•Š ğŸ˜
--                            =âŸ¨âŸ©
--                              â€µfun suc (âˆ™ , â€µfun zero âˆ™)
--                            =âŸ¨ â€µcong suc zero refl refl
--                                  (begin
--                                    â€µfun zero âˆ™
--                                  =Ë˜âŸ¨ â€µcomp zero âˆ™ refl âŸ©
--                                    â€µfun (comp zero âˆ™) (tab â€µvar)
--                                  âˆ)
--                                âŸ©
--                              â€µfun suc (âˆ™ , â€µfun (comp zero âˆ™) (tab â€µvar))
--                            =Ë˜âŸ¨ â€µcomp suc ((âˆ™ , comp zero âˆ™)) refl âŸ©
--                              â€µfun (comp suc (âˆ™ , comp zero âˆ™)) (tab â€µvar)
--                            =âŸ¨âŸ©
--                              â€µfun (Æ’const 1) (tab â€µvar)
--                            =âŸ¨ 0 âŸ©
--                              ğŸ˜
--                            âˆ
--   lem3 (t â€µ= u) = {!!}


----------------------------------------------------------------------------------------------------

-- Î â°â‚‚ class of formulas

-- TODO: definition of Î â°â‚‚
-- TODO: lemma 4


----------------------------------------------------------------------------------------------------

-- double negation translation

_Â° : âˆ€ {k} â†’ Fm k â†’ Fm k
(A â€µâŠƒ B) Â° = A Â° â€µâŠƒ B Â°
(A â€µâˆ§ B) Â° = A Â° â€µâˆ§ B Â°
(A â€µâˆ¨ B) Â° = â€µÂ¬ â€µÂ¬ (A Â° â€µâˆ¨ B Â°)
(â€µâˆ€ A)   Â° = â€µâˆ€ A Â°
(â€µâˆƒ A)   Â° = â€µÂ¬ â€µÂ¬ (â€µâˆƒ A Â°)
â€µâŠ¥      Â° = â€µâŠ¥
(t â€µ= u) Â° = â€µÂ¬ â€µÂ¬ (t â€µ= u)

_Â°Â§ : âˆ€ {k} â†’ FmÂ§ k â†’ FmÂ§ k
âˆ™       Â°Â§ = âˆ™
(Î“ , A) Â°Â§ = Î“ Â°Â§ , A Â°

-- TODO: interactions between DNT and renaming/substitution
module _ where
  postulate
    TODO1 : âˆ€ {k} {A : Fm (suc k)} {t} â†’ A Â° [ t /0]Fm â‰¡ A [ t /0]Fm Â°
  -- TODO1 = {!!}

  postulate
    TODO2 : âˆ€ {Ã k} {Î“ : FmÂ§ k} {A} â†’ Ã / wkFmÂ§ Î“ Â°Â§ âŠ¢ A â†’ Ã / wkFmÂ§ (Î“ Â°Â§) âŠ¢ A
  -- TODO2 = {!!}

  postulate
    TODO3 : âˆ€ {Ã k} {Î“ : FmÂ§ k} {A t} â†’ Ã / Î“ âŠ¢ A [ t /0]Fm Â° â†’ Ã / Î“ âŠ¢ A Â° [ t /0]Fm
  -- TODO3 = {!!}

  postulate
    TODO4 : âˆ€ {Ã k} {Î“ : FmÂ§ k} {A t} â†’ Ã / Î“ âŠ¢ â€µâˆ€ (A Â° â€µâŠƒ wkFm A [ t /1]Fm Â°) â†’
              Ã / Î“ âŠ¢ â€µâˆ€ (A Â° â€µâŠƒ wkFm (A Â°) [ t /1]Fm)
  -- TODO4 = {!!}

  postulate
    TODO5 : âˆ€ {Ã k} {Î“ : FmÂ§ k} {A C} â†’ Ã / wkFmÂ§ Î“ Â°Â§ , A Â° âŠ¢ wkFm C Â° â†’
              Ã / wkFmÂ§ (Î“ Â°Â§) , A Â° âŠ¢ wkFm (C Â°)
  -- TODO5 = {!!}

-- TODO: lemma 5
module _ where
  open â«—-Reasoning

  lem5-1 : âˆ€ {k} {Î“ : FmÂ§ k} {A} â†’ PA / Î“ âŠ¢ A Â° â€µâ«— A
  lem5-1 {A = A â€µâŠƒ B} = â€µcongâŠƒ lem5-1 lem5-1
  lem5-1 {A = A â€µâˆ§ B} = â€µcongâˆ§ lem5-1 lem5-1
  lem5-1 {A = A â€µâˆ¨ B} = begin
                          (A â€µâˆ¨ B) Â°
                        â«—âŸ¨ â€µdn âŸ©
                          A Â° â€µâˆ¨ B Â°
                        â«—âŸ¨ â€µcongâˆ¨ lem5-1 lem5-1 âŸ©
                          A â€µâˆ¨ B
                        âˆ
  lem5-1 {A = â€µâˆ€ A}   = â€µcongâˆ€ lem5-1
  lem5-1 {A = â€µâˆƒ A}   = begin
                          (â€µâˆƒ A) Â°
                        â«—âŸ¨ â€µdn âŸ©
                          â€µâˆƒ A Â°
                        â«—âŸ¨ â€µcongâˆƒ lem5-1 âŸ©
                          â€µâˆƒ A
                        âˆ
  lem5-1 {A = â€µâŠ¥}    = â«—refl
  lem5-1 {A = t â€µ= u} = â€µdn

lem5-2 : âˆ€ {Ã k} {Î“ : FmÂ§ k} {A} â†’ Ã / Î“ âŠ¢ â€µÂ¬ â€µÂ¬ (A Â°) â€µâŠƒ A Â°
lem5-2 {A = A â€µâŠƒ B} = â€µlam (â€µlam (lem5-2 â€µ$ â€µlam
                         (2 â€µ$ â€µlam
                           (1 â€µ$ 0 â€µ$ 2))))
lem5-2 {A = A â€µâˆ§ B} = â€µlam (â€µpair
                         (lem5-2 â€µ$ â€µlam
                           (1 â€µ$ â€µlam
                             (1 â€µ$ â€µfst 0)))
                         (lem5-2 â€µ$ â€µlam
                           (1 â€µ$ â€µlam
                             (1 â€µ$ â€µsnd 0))))
lem5-2 {A = A â€µâˆ¨ B} = â€µlam (â€µjoin 0)
lem5-2 {A = â€µâˆ€ A}   = â€µlam (â€µall refl (lem5-2 â€µ$ â€µlam
                         (1 â€µ$ â€µlam
                           (1 â€µ$ â€µunall (â€µtvar 0) (idcutFm (A Â°)) 0))))
lem5-2 {A = â€µâˆƒ A}   = â€µlam (â€µjoin 0)
lem5-2 {A = â€µâŠ¥}    = â€µlam (0 â€µ$ âŠƒid)
lem5-2 {A = t â€µ= u} = â€µlam (â€µjoin 0)

lem5-3âˆ‹ : âˆ€ {k} {Î“ : FmÂ§ k} {A} â†’ Î“ âˆ‹ A â†’ Î“ Â°Â§ âˆ‹ A Â°
lem5-3âˆ‹ zero    = zero
lem5-3âˆ‹ (suc i) = suc (lem5-3âˆ‹ i)

-- TODO: why does rewriting blow up constraint solver here?
module _ where
  lem5-3 : âˆ€ {Ã k} {Î“ : FmÂ§ k} {A} â†’ PA / Î“ âŠ¢ A â†’ Ã / Î“ Â°Â§ âŠ¢ A Â°
  lem5-3 (â€µvar i)                = â€µvar (lem5-3âˆ‹ i)
  lem5-3 (â€µlam d)                = â€µlam (lem5-3 d)
  lem5-3 (d â€µ$ e)                = lem5-3 d â€µ$ lem5-3 e
  lem5-3 (â€µpair d e)             = â€µpair (lem5-3 d) (lem5-3 e)
  lem5-3 (â€µfst d)                = â€µfst (lem5-3 d)
  lem5-3 (â€µsnd d)                = â€µsnd (lem5-3 d)
  lem5-3 (â€µleft d)               = â€µreturn (â€µleft (lem5-3 d))
  lem5-3 (â€µright d)              = â€µreturn (â€µright (lem5-3 d))
  lem5-3 (â€µeither c d e)         = lem5-2 â€µ$ (lem5-3 c â€µ>>= â€µlam (â€µeither 0
                                     (â€µreturn (â€µexch (wk (lem5-3 d))))
                                     (â€µreturn (â€µexch (wk (lem5-3 e))))))
  lem5-3 {Î“ = Î“} (â€µall refl d)
      = â€µall refl (TODO2 {Î“ = Î“} (lem5-3 d))

  lem5-3 (â€µunall t refl d)       = â€µunall t TODO1 (lem5-3 d)
  lem5-3 (â€µex t refl d)          = â€µreturn (â€µex t TODO1 (lem5-3 d))

  lem5-3 {Î“ = Î“} (â€µletex {C = C} refl refl d e)
      = lem5-2 â€µ$
          (lem5-3 d â€µ>>=
            â€µlam (â€µletex refl refl 0
              (â€µreturn (â€µexch (wk (TODO5 {Î“ = Î“} {C = C} (lem5-3 e)))))))

  lem5-3 (â€µmagicPA d)            = lem5-2 â€µ$ â€µlam (lem5-3 d)
  lem5-3 â€µrefl                   = â€µreturn â€µrefl
  lem5-3 (â€µsym d)                = lem5-3 d â€µ>>= â€µlam
                                     (â€µreturn (â€µsym 0))
  lem5-3 (â€µtrans d e)            = lem5-3 d â€µ>>= â€µlam
                                     (wk (lem5-3 e) â€µ>>= â€µlam
                                       (â€µreturn (â€µtrans 1 0)))
  lem5-3 (â€µcong f i refl refl d) = lem5-3 d â€µ>>= â€µlam
                                     (â€µreturn (â€µcong f i refl refl 0))
  lem5-3 â€µdis                    = â€µreturn â€µdis
  lem5-3 (â€µinj d)                = lem5-3 d â€µ>>= â€µlam
                                     (â€µreturn (â€µinj 0))
  lem5-3 (â€µind refl refl d e)    = â€µind refl refl (TODO3 (lem5-3 d)) (TODO4 (lem5-3 e))
  lem5-3 (â€µproj i refl)          = â€µreturn (â€µproj i refl)
  lem5-3 (â€µcomp g Ï† refl)        = â€µreturn (â€µcomp g Ï† refl)
  lem5-3 (â€µrec {t = t} f g)      = â€µpair
                                     (â€µreturn (â€µfst (â€µrec {t = t} f g)))
                                     (â€µreturn (â€µsnd (â€µrec f g)))

-- "Note that the converse of 3 trivially holds wih 1."
lem5-3â»Â¹ : âˆ€ {Ã k} {Î“ : FmÂ§ k} {A} â†’ Ã / Î“ Â°Â§ âŠ¢ A Â° â†’ PA / Î“ âŠ¢ A
lem5-3â»Â¹ d = aux (â€µfst lem5-1 â€µ$ lem2 d)
  where
    aux : âˆ€ {k} {Î“ : FmÂ§ k} {A} â†’ PA / Î“ Â°Â§ âŠ¢ A â†’ PA / Î“ âŠ¢ A
    aux {Î“ = âˆ™}     d = d
    aux {Î“ = Î“ , C} d = wk (aux (â€µlam d)) â€µ$ (â€µsnd lem5-1 â€µ$ 0)

-- TODO: "A counterexample for 4 is Â¬âˆ€y.A[y/xâ‚€]."
-- lem5-4 : âˆ€ {k} {Î“ : FmÂ§ k} â†’ Â¬ (âˆ€ {A} â†’ HA / Î“ , â€µÂ¬ (â€µâˆ€ A) âŠ¢ (â€µÂ¬ (â€µâˆ€ A)) Â°)
-- lem5-4 = {!!}


----------------------------------------------------------------------------------------------------

-- A-translation

_á´¬âŸ¨_âŸ© : âˆ€ {k} â†’ Fm k â†’ Fm k â†’ Fm k
(A â€µâŠƒ B) á´¬âŸ¨ T âŸ© = A á´¬âŸ¨ T âŸ© â€µâŠƒ B á´¬âŸ¨ T âŸ©
(A â€µâˆ§ B) á´¬âŸ¨ T âŸ© = A á´¬âŸ¨ T âŸ© â€µâˆ§ B á´¬âŸ¨ T âŸ©
(A â€µâˆ¨ B) á´¬âŸ¨ T âŸ© = A á´¬âŸ¨ T âŸ© â€µâˆ¨ B á´¬âŸ¨ T âŸ©
(â€µâˆ€ A)   á´¬âŸ¨ T âŸ© = â€µâˆ€ A á´¬âŸ¨ wkFm T âŸ©
(â€µâˆƒ A)   á´¬âŸ¨ T âŸ© = â€µâˆƒ A á´¬âŸ¨ wkFm T âŸ©
â€µâŠ¥      á´¬âŸ¨ T âŸ© = T
(t â€µ= u) á´¬âŸ¨ T âŸ© = (t â€µ= u) â€µâˆ¨ T

_á´¬âŸ¨_âŸ©Â§ : âˆ€ {k} â†’ FmÂ§ k â†’ Fm k â†’ FmÂ§ k
âˆ™       á´¬âŸ¨ T âŸ©Â§ = âˆ™
(Î“ , A) á´¬âŸ¨ T âŸ©Â§ = Î“ á´¬âŸ¨ T âŸ©Â§ , A á´¬âŸ¨ T âŸ©

-- TODO: interactions between A-translation and renaming/substitution
module _ where
  postulate
    TODO6 : âˆ€ {k} {A : Fm (suc k)} {T t} â†’ (A á´¬âŸ¨ wkFm T âŸ©) [ t /0]Fm â‰¡ (A [ t /0]Fm) á´¬âŸ¨ T âŸ©
  -- TODO6 = ?

-- TODO: lemma 6
module _ where
  open â‰¡

  -- non-constructive lemma
  aux1 : âˆ€ {k} {Î“ : FmÂ§ k} {A B C} â†’ PA / Î“ âŠ¢ (A â€µâˆ¨ C) â€µâŠƒ (B â€µâˆ¨ C) â€µâ«— (A â€µâŠƒ B) â€µâˆ¨ C
  aux1 = â€µpair
           (â€µlam (â€µeither â€µem
             (â€µright 0)
             (â€µleft (â€µlam
               (â€µeither (2 â€µ$ (â€µleft 0))
                 0
                 (â€µabort (2 â€µ$ 0)))))))
           (â€µlam (â€µlam (â€µeither 0
             (â€µeither 2
               (â€µleft (0 â€µ$ 1))
               (â€µright 0))
             (â€µright 0))))

  aux2 : âˆ€ {Ã k} {Î“ : FmÂ§ k} {A B C} â†’ Ã / Î“ âŠ¢ (A â€µâˆ¨ C) â€µâˆ§ (B â€µâˆ¨ C) â€µâ«— (A â€µâˆ§ B) â€µâˆ¨ C
  aux2 = â€µpair
           (â€µlam (â€µeither (â€µfst 0)
             (â€µeither (â€µsnd 1)
               (â€µleft (â€µpair 1 0))
               (â€µright 0))
             (â€µright 0)))
           (â€µlam (â€µeither 0
             (â€µpair (â€µleft (â€µfst 0)) (â€µleft (â€µsnd 0)))
             (â€µpair (â€µright 0) (â€µright 0))))

  aux3 : âˆ€ {Ã k} {Î“ : FmÂ§ k} {A B C} â†’ Ã / Î“ âŠ¢ (A â€µâˆ¨ C) â€µâˆ¨ (B â€µâˆ¨ C) â€µâ«— (A â€µâˆ¨ B) â€µâˆ¨ C
  aux3 = â€µpair
           (â€µlam (â€µeither 0
             (â€µeither 0
               (â€µleft (â€µleft 0))
               (â€µright 0))
             (â€µeither 0
               (â€µleft (â€µright 0))
               (â€µright 0))))
           (â€µlam (â€µeither 0
             (â€µeither 0
               (â€µleft (â€µleft 0))
               (â€µright (â€µleft 0)))
             (â€µleft (â€µright 0)))) -- could also be â€µright

  -- non-constructive lemma
  aux4 : âˆ€ {k} {Î“ : FmÂ§ k} {A C} â†’ PA / Î“ âŠ¢ â€µâˆ€ (A â€µâˆ¨ wkFm C) â€µâ«— â€µâˆ€ A â€µâˆ¨ C
  aux4 {A = A} {C} = â€µpair
                       (â€µlam (â€µeither â€µem
                         (â€µright 0)
                         (â€µleft
                           (â€µall refl (â€µeither (â€µunall (â€µtvar 0) (idcutFm (A â€µâˆ¨ wkFm C)) 1)
                             0
                             (â€µabort (1 â€µ$ 0)))))))
                       (â€µlam (â€µeither 0
                         (â€µall refl (â€µleft (â€µunall (â€µtvar 0) (idcutFm A) 0)))
                         (â€µall refl (â€µright 0))))

  aux5 : âˆ€ {Ã k} {Î“ : FmÂ§ k} {A C} â†’ Ã / Î“ âŠ¢ â€µâˆƒ (A â€µâˆ¨ wkFm C) â€µâ«— â€µâˆƒ A â€µâˆ¨ C
  aux5 {A = A} {C} = â€µpair
                       (â€µlam (â€µletex refl refl 0 (â€µeither 0
                         (â€µleft (â€µex (â€µtvar 0) (idcutFm A) 0))
                         (â€µright 0))))
                       (â€µlam (â€µeither 0
                         (â€µletex refl refl 0
                           (â€µex (â€µtvar 0) (_â€µâˆ¨_ & idcutFm A âŠ— idcutFm (wkFm C)) (â€µleft 0)))
                         (â€µex ğŸ˜ -- could also be any other natural
                           ( (subFm (idTmÂ§ , ğŸ˜) A â€µâˆ¨_)
                               & ( eqsubFm idTmÂ§ ğŸ˜ C
                                 â‹® idsubFm C
                                 )
                           )
                           (â€µright 0))))

  aux6 : âˆ€ {Ã k} {Î“ : FmÂ§ k} {C} â†’ Ã / Î“ âŠ¢ C â€µâ«— â€µâŠ¥ â€µâˆ¨ C
  aux6 = â€µpair
           (â€µlam (â€µright 0))
           (â€µlam (â€µeither 0 (â€µabort 0) 0))

module _ where
  open â«—-Reasoning

  lem6-1 : âˆ€ {k} {Î“ : FmÂ§ k} {A T} â†’ PA / Î“ âŠ¢ A á´¬âŸ¨ T âŸ© â€µâ«— A â€µâˆ¨ T
  lem6-1 {A = A â€µâŠƒ B} {T} = begin
                              A á´¬âŸ¨ T âŸ© â€µâŠƒ B á´¬âŸ¨ T âŸ©
                            â«—âŸ¨ â€µcongâŠƒ lem6-1 lem6-1 âŸ©
                              (A â€µâˆ¨ T) â€µâŠƒ (B â€µâˆ¨ T)
                            â«—âŸ¨ aux1 âŸ©
                              (A â€µâŠƒ B) â€µâˆ¨ T
                            âˆ
  lem6-1 {A = A â€µâˆ§ B} {T} = begin
                              A á´¬âŸ¨ T âŸ© â€µâˆ§ B á´¬âŸ¨ T âŸ©
                            â«—âŸ¨ â€µcongâˆ§ lem6-1 lem6-1 âŸ©
                              (A â€µâˆ¨ T) â€µâˆ§ (B â€µâˆ¨ T)
                            â«—âŸ¨ aux2 âŸ©
                              (A â€µâˆ§ B) â€µâˆ¨ T
                            âˆ
  lem6-1 {A = A â€µâˆ¨ B} {T} = begin
                              A á´¬âŸ¨ T âŸ© â€µâˆ¨ B á´¬âŸ¨ T âŸ©
                            â«—âŸ¨ â€µcongâˆ¨ lem6-1 lem6-1 âŸ©
                              (A â€µâˆ¨ T) â€µâˆ¨ (B â€µâˆ¨ T)
                            â«—âŸ¨ aux3 âŸ©
                              (A â€µâˆ¨ B) â€µâˆ¨ T
                            âˆ
  lem6-1 {A = â€µâˆ€ A}   {T} = begin
                              â€µâˆ€ (A á´¬âŸ¨ wkFm T âŸ©)
                            â«—âŸ¨ â€µcongâˆ€ lem6-1 âŸ©
                              â€µâˆ€ (A â€µâˆ¨ wkFm T)
                            â«—âŸ¨ aux4 âŸ©
                              â€µâˆ€ A â€µâˆ¨ T
                            âˆ
  lem6-1 {A = â€µâˆƒ A}   {T} = begin
                              â€µâˆƒ (A á´¬âŸ¨ wkFm T âŸ©)
                            â«—âŸ¨ â€µcongâˆƒ lem6-1 âŸ©
                              â€µâˆƒ (A â€µâˆ¨ wkFm T)
                            â«—âŸ¨ aux5 âŸ©
                              â€µâˆƒ A â€µâˆ¨ T
                            âˆ
  lem6-1 {A = â€µâŠ¥}    {T} = aux6
  lem6-1 {A = t â€µ= u} {T} = â«—refl

-- lem6-2 : âˆ€ {Ã k} {Î“ : FmÂ§ k} {A T} â†’ Ã / Î“ âŠ¢ T â€µâŠƒ A á´¬âŸ¨ T âŸ©
-- lem6-2 {A = A â€µâŠƒ B}    = â€µlam (â€µlam (lem6-2 â€µ$ 1)) -- function argument ignored
-- lem6-2 {A = A â€µâˆ§ B}    = â€µlam (â€µpair (lem6-2 â€µ$ 0) (lem6-2 â€µ$ 0))
-- lem6-2 {A = A â€µâˆ¨ B}    = â€µlam (â€µleft (lem6-2 â€µ$ 0)) -- could also be â€µright
-- lem6-2 {A = â€µâˆ€ A}      = â€µlam (â€µall refl (lem6-2 â€µ$ 0))
-- lem6-2 {A = â€µâˆƒ A}  {T} = {!!}
-- -- â€µlam (â€µex ğŸ˜ (TODO6 {A = A} {T}) (lem6-2 {A = A [ ğŸ˜ /0]Fm} â€µ$ 0)) -- TODO: termination failure
-- lem6-2 {A = â€µâŠ¥}       = âŠƒid
-- lem6-2 {A = t â€µ= u}    = â€µlam (â€µright 0)
--
-- lem6-3âˆ‹ : âˆ€ {k} {Î“ : FmÂ§ k} {A T} â†’ Î“ âˆ‹ A â†’ Î“ á´¬âŸ¨ T âŸ©Â§ âˆ‹ A á´¬âŸ¨ T âŸ©
-- lem6-3âˆ‹ zero    = zero
-- lem6-3âˆ‹ (suc i) = suc (lem6-3âˆ‹ i)

-- TODO: "The proof of 3 is a bit tricky where eigenvariable conditions are involved."
-- lem6-3 : âˆ€ {Ã k} {Î“ : FmÂ§ k} {A T} â†’ Ã / Î“ âŠ¢ A â†’ Ã / Î“ á´¬âŸ¨ T âŸ©Â§ âŠ¢ A á´¬âŸ¨ T âŸ©
-- lem6-3 (â€µvar i)                = â€µvar (lem6-3âˆ‹ i)
-- lem6-3 (â€µlam d)                = â€µlam (lem6-3 d)
-- lem6-3 (d â€µ$ e)                = lem6-3 d â€µ$ lem6-3 e
-- lem6-3 (â€µpair d e)             = â€µpair (lem6-3 d) (lem6-3 e)
-- lem6-3 (â€µfst d)                = â€µfst (lem6-3 d)
-- lem6-3 (â€µsnd d)                = â€µsnd (lem6-3 d)
-- lem6-3 (â€µleft d)               = â€µleft (lem6-3 d)
-- lem6-3 (â€µright d)              = â€µright (lem6-3 d)
-- lem6-3 (â€µeither c d e)         = â€µeither (lem6-3 c) (lem6-3 d) (lem6-3 e)
-- lem6-3 (â€µall refl d)           = {!!}
-- lem6-3 (â€µunall t refl d)       = {!!}
-- lem6-3 (â€µex t refl d)          = {!!}
-- lem6-3 (â€µletex refl refl d e)  = {!!}
-- lem6-3 (â€µabort d)              = {!!}
-- lem6-3 (â€µmagic d)              = {!!}
-- lem6-3 â€µrefl                   = â€µleft â€µrefl
-- lem6-3 (â€µsym d)                = â€µeither (lem6-3 d)
--                                    (â€µleft (â€µsym 0))
--                                    (â€µright 0)
-- lem6-3 (â€µtrans d e)            = â€µeither (lem6-3 d)
--                                    (â€µeither (wk (lem6-3 e))
--                                      (â€µleft (â€µtrans 1 0))
--                                      (â€µright 0))
--                                    (â€µright 0)
-- lem6-3 (â€µcong f i refl refl d) = {!!}
-- lem6-3 â€µdis                    = {!!}
-- lem6-3 (â€µinj d)                = {!!}
-- lem6-3 (â€µind refl refl d e)    = {!!}
-- lem6-3 (â€µproj i refl)          = {!!}
-- lem6-3 (â€µcomp g Ï† refl)        = {!!}
-- lem6-3 (â€µrec f g)              = {!!}

-- TODO: "A counterexample for 4 is A = Â¬Â¬T."
-- lem6-4 : âˆ€ {k} {Î“ : FmÂ§ k} â†’ Â¬ (âˆ€ {T} â†’ HA / Î“ , â€µÂ¬ â€µÂ¬ T âŠ¢ (â€µÂ¬ â€µÂ¬ T) á´¬âŸ¨ T âŸ©)
-- lem6-4 = {!!}


----------------------------------------------------------------------------------------------------

-- proof of theorem 1

-- TODO: lemma 7
-- TODO: corollary 8
-- TODO: theorem 1


----------------------------------------------------------------------------------------------------
```

Lorem ipsum dolor sit amet, consectetur adipisicing elit, sed do eiusmod tempor incididunt ut labore
et dolore magna aliqua.  Ut enim ad minim veniam, quis nostrud exercitation ullamco laboris nisi ut
aliquip ex ea commodo consequat. Duis aute irure dolor in reprehenderit in voluptate velit esse
cillum dolore eu fugiat nulla pariatur. Excepteur sint occaecat cupidatat non proident, sunt in
culpa qui officia deserunt mollit anim id est laborum.
